More work in Lambda.v

Instance/Lambda.v
@@ -1,5 +1,9 @@
 Set Warnings "-notation-overridden".
 
+Require Import Equations.Equations.
+Require Import Equations.EqDec.
+Unset Equations WithK.
+
 Require Import Category.Lib.
 Require Export Category.Theory.Functor.
 
@@ -14,6 +18,8 @@ Set Decidable Equality Schemes.
 Inductive type : Set :=
   | Ty : type
   | Func : type -> type -> type.
+
+Derive NoConfusion Subterm EqDec for type.
 
 Notation "x --> y" := (Func x y) (at level 55, right associativity) : type_scope.
 
@@ -39,6 +45,8 @@ Inductive preterm : Set :=
   | Abs (d : type) (body : preterm)
   | App (arg body : preterm).
 
+Derive NoConfusion Subterm EqDec for preterm.
+
 Notation "% x" := (Var x) (at level 20).
 Infix "@" := App (at level 25, left associativity).
 Notation "\ A => M" := (Abs A M) (at level 35).
@@ -58,6 +66,7 @@ Notation "E |= x :!"   := (VarUD E x) (at level 60).
 Definition decl (A : type) E := Some A :: E.
 
 Infix "[#]" := decl (at level 20, right associativity).
+Notation "E ∪ { A }" := (decl A E) (at level 20, right associativity).
 
 Inductive Typing : Env -> preterm -> type -> Set :=
   | TVar: ∀ Γ x α,                            (* x : α ∈ Γ *)
@@ -65,7 +74,7 @@ Inductive Typing : Env -> preterm -> type -> Set :=
       -> Γ |- %x := α                         (* Γ ⊢ x : α *)
 
   | TAbs: ∀ Γ α β t,                          (*  Γ ∪ {x : α} ⊢ t : β  *)
-         α [#] Γ |- t := β                    (* --------------------- *)
+         Γ ∪ {α} |- t := β                    (* --------------------- *)
       -> Γ |- \α => t := α --> β              (* Γ ⊢ λx : α. t : α → β *)
 
   | TApp: ∀ Γ α β t u,                        (* Γ ⊢ t : α → β   Γ ⊢ u : α *)
@@ -74,6 +83,8 @@ Inductive Typing : Env -> preterm -> type -> Set :=
 
   where "Γ |- t := α" := (Typing Γ t α).
 
+Derive NoConfusion Signature for Typing.
+
 Record term : Set := mkterm {
   env    : Env;
   tm     : preterm;
@@ -81,14 +92,14 @@ Record term : Set := mkterm {
   typing : Typing env tm ty
 }.
 
-Lemma Type_unique : ∀ Pt E T1 T2
-  (D1 : Typing E Pt T1) (D2 : Typing E Pt T2), T1 = T2.
+Lemma Type_unique : ∀ t E T1 T2
+  (D1 : Typing E t T1) (D2 : Typing E t T2), T1 = T2.
 Proof.
   intros.
   generalize dependent E.
   generalize dependent T1.
   generalize dependent T2.
-  induction Pt; simpl; intros.
+  induction t; simpl; intros.
   - inversion_clear D1.
     inversion H; subst; clear H.
     inversion_clear D2.
@@ -98,25 +109,44 @@ Proof.
   - inversion_clear D1.
     inversion_clear D2.
     f_equal.
-    now eapply IHPt; eauto.
+    now eapply IHt; eauto.
   - inversion_clear D1.
     inversion_clear D2.
-    specialize (IHPt1 _ _ _ H H1).
-    specialize (IHPt2 _ _ _ H0 H2).
+    specialize (IHt1 _ _ _ H H1).
+    specialize (IHt2 _ _ _ H0 H2).
     subst.
-    now inversion_clear IHPt1.
+    now inversion_clear IHt1.
 Qed.
 
-Lemma typing_unique : ∀ E Pt T (D1 D2 : Typing E Pt T),
-  D1 = D2.
+Definition option_dec {A} (H : ∀ a b : A, {a = b} + {a <> b}) :
+  ∀ a b : option A, {a = b} + {a <> b}.
+Proof.
+  decide equality.
+Defined.
+
+Lemma typing_unique : ∀ E t T (D1 D2 : Typing E t T), D1 = D2.
 Proof.
   intros.
-  apply Eqdep_dec.eq_dep_eq_dec.
-    apply type_eq_dec.
-Admitted.
+  induction D1.
+  - dependent elimination D2.
+    f_equal.
+    apply Eqdep_dec.UIP_dec; intros.
+    apply option_dec; intros.
+    apply option_dec; intros.
+    now apply type_eq_dec.
+  - dependent elimination D2.
+    f_equal.
+    now apply IHD1.
+  - dependent elimination D2.
+    pose proof (Type_unique _ _ _ _ D1_1 t3).
+    pose proof (Type_unique _ _ _ _ D1_2 t4).
+    subst.
+    f_equal.
+      now apply IHD1_1.
+    now apply IHD1_2.
+Qed.
 
-Lemma term_eq : ∀ M N,
-  env M = env N -> tm M = tm N -> M = N.
+Lemma term_eq : ∀ M N, env M = env N -> tm M = tm N -> M = N.
 Proof.
   intros.
   destruct M, N; simpl in *; subst.
@@ -125,243 +155,30 @@ Proof.
   apply typing_unique.
 Qed.
 
-Theorem autoType E Pt :
-  { N : term | env N = E & tm N = Pt} +
-  { ~ exists N : term, env N = E /\ tm N = Pt}.
+Program Definition identity (Γ : Env) (x : type) :
+  Typing Γ (\x => %0) (x --> x) :=
+  TAbs _ _ _ _ (TVar _ _ _ _).
+
+Definition composition (Γ : Env) (x y z : type) (f g : preterm)
+           (Tf : Typing Γ f (y --> z))
+           (Tg : Typing Γ g (x --> y)) :
+  Typing Γ (\x => f @ (g @ %0)) (x --> z).
 Proof.
-(*
-  destruct ({ α : type & Typing E Pt α } + { ~ exists α : type, Typing E Pt α }).
-  generalize dependent E.
-
-  induction Pt; intros.
-  - left.
-    exists {| env := E; tm := %i; ty := Ty; typing := TVar _ _ _ |}.
-*)
-Abort.
-
-Inductive Scope (var : type -> Type) (t : type) : type -> Type :=
-  | Here : Scope var t t
-  | Next u : var u -> Scope var t u.
-
-Arguments Here {_ _}.
-Arguments Next {_ _ _} _.
-
-Fixpoint scope_map {var var' : type -> Type} (f : ∀ t, var t -> var' t)
-        {d ty} (e : Scope var d ty) : Scope var' d ty :=
-  match e with
-  | Here => Here
-  | Next x => Next (f _ x)
-  end.
-
-Arguments Var {var _} _.
-Arguments Abs {var _ _} _.
-Arguments App {var _ _} _ _.
-
-Fixpoint lam_size {var : type -> Type} {ty} (e : Lam var ty) : nat :=
-  match e with
-  | Var x => 1
-  | Abs x => 1 + lam_size x
-  | App func arg => 1 + lam_size func + lam_size arg
-  end.
-
-Fixpoint lam_map {var var' : type -> Type} (f : ∀ t, var t -> var' t)
-         {ty} (e : Lam var ty) : Lam var' ty :=
-  match e with
-  | Var x => Var (f _ x)
-  | Abs x => Abs (lam_map (fun _ => scope_map f) x)
-  | App func arg => App (lam_map f func) (lam_map f arg)
-  end.
-
-Lemma lam_map_size {var var' : type -> Type}
-      (f : ∀ t, var t -> var' t) {ty} (e : Lam var ty) :
-  lam_size (lam_map f e) = lam_size e.
-Proof.
-  generalize dependent var'.
-  induction e; simpl; auto.
-Defined.
-
-(** Instantiating a bound variable is function application. *)
-
-Definition instantiate {var : type -> Type}
-           {d c} (v : var d) (e : Lam (Scope var d) c) : Lam var c :=
-  let go _ x :=
-      match x with
-      | Here => v
-      | Next x => x
-      end in
-  lam_map go e.
-
-Corollary instantiate_size {var : type -> Type} {d c} (v : var d)
-          (e : Lam (Scope var d) c) :
-  lam_size (instantiate v e) = lam_size e.
-Proof.
-  unfold instantiate.
-  apply lam_map_size.
-Defined.
-
-Import EqNotations.
-
-Ltac simpl_eq :=
-  unfold eq_rect_r, eq_rect, eq_ind_r, eq_ind, eq_sym, prod_rect,
-         EqdepFacts.internal_eq_rew_r_dep,
-         EqdepFacts.internal_eq_sym_involutive,
-         EqdepFacts.internal_eq_sym_internal in *.
-
-Program Fixpoint lamD {t : type} (var : type -> Type)
-        (e : Lam (typeD var) t) {measure (lam_size e)} : typeD var t :=
-  match e as e' in Lam _ t'
-  return ∀ H : t' = t, e' = rew <- H in e -> typeD var t' with
-  | Var x        => fun _ _ => x
-  | Abs body     => fun _ _ => fun arg => lamD var (instantiate arg body)
-  | App func arg => fun _ _ => lamD var func (lamD var arg)
-  end eq_refl eq_refl.
-Next Obligation.
-  rewrite instantiate_size.
-  simpl_eq; subst; simpl; abstract omega.
-Defined.
-Next Obligation. simpl_eq; subst; simpl; abstract omega. Defined.
-Next Obligation. simpl_eq; subst; simpl; abstract omega. Defined.
-
-(* ∀ (f : () -> ()) (t : ()), f t : () *)
-Definition example1 :
-  Lam (fun _ => nat) (Func Ty (Func Ty Ty)) :=
-  Abs (Abs (App (Abs (Var Here)) (Var Here))).
-
-Notation "^" := Var.
-Infix "@" := App (left associativity, at level 50).
-Notation "\ x : t , e" :=
-  (@Abs _ t _ e) (no associativity, at level 51, x at level 0, only parsing).
-
-(*
-Eval cbv beta iota delta zeta in
-    lamD (fun _ => Datatypes.unit) ((\x : Ty, ^Here) @ ^tt).
-
-Eval cbv beta iota delta zeta in
-    lamD (fun _ => Datatypes.nat) (@Abs _ Ty Ty (^(Next 5%nat)) @ ^5%nat).
-*)
-
-Require Import Coq.Strings.String.
-
-Open Scope string_scope.
-
-Inductive ty : Type :=
-  | Name : string -> ty
-  | Func : ty → ty → ty.
-
-Inductive tm : Type :=
-  | var : string → tm
-  | app : tm → tm → tm
-  | abs : string → ty → tm → tm.
-
-Inductive value : tm → Prop :=
-  | v_abs : ∀ x T t,
-      value (abs x T t).
-
-Hint Constructors value.
-
-Reserved Notation "'[' x ':=' s ']' t" (at level 20).
-
-Fixpoint subst (x:string) (s:tm) (t:tm) : tm :=
-  match t with
-  | var x' =>
-      if string_dec x x' then s else t
-  | abs x' T t1 =>
-      abs x' T (if string_dec x x' then t1 else ([x:=s] t1))
-  | app t1 t2 =>
-      app ([x:=s] t1) ([x:=s] t2)
-  end
-
-where "'[' x ':=' s ']' t" := (subst x s t).
-
- Inductive substi (s:tm) (x:string) : tm → tm → Prop :=
-  | s_var1 :
-      substi s x (var x) s
-  | s_var2 : ∀ x0,
-      substi s x (var x0) (var x0)
-  | s_abs : ∀ T t1,
-      substi s x (abs x T t1) s
-  | s_app : ∀ t1 t2,
-      substi s x (app t1 t2) s.
-
-Hint Constructors substi.
-
-Theorem substi_correct : ∀ s x t t',
-  [x:=s]t = t' ↔ substi s x t t'.
-Proof.
-  split; intros.
-  - induction t.
-    + simpl in H.
-      destruct (string_dec x s0); subst.
-        constructor.
-      constructor.
+  constructor.
+  apply TApp with (α := y); auto.
+    admit.
+  apply TApp with (α := x); auto.
+    admit.
+  apply TVar.
+  constructor.
 Admitted.
-
-Reserved Notation "t1 '===>' t2" (at level 40).
-
-Inductive step : tm → tm → Prop :=
-  | ST_AppAbs : ∀ x T t12 v2,
-         value v2 →
-         (app (abs x T t12) v2) ===> [x:=v2]t12
-  | ST_App1 : ∀ t1 t1' t2,
-         t1 ===> t1' →
-         app t1 t2 ===> app t1' t2
-  | ST_App2 : ∀ v1 t2 t2',
-         value v1 →
-         t2 ===> t2' →
-         app v1 t2 ===> app v1 t2'
-
-where "t1 '===>' t2" := (step t1 t2).
-
-Hint Constructors step.
-
-(* Notation multistep := (multi step). *)
-(* Notation "t1 '===>*' t2" := (multistep t1 t2) (at level 40). *)
-
-Reserved Notation "Gamma '|-' t '∈' T" (at level 40).
-
-Inductive has_type : context → tm → ty → Prop :=
-  | T_Var : ∀ Gamma x T,
-      Gamma x = Some T →
-      Gamma |- tvar x ∈ T
-  | T_Abs : ∀ Gamma x T11 T12 t12,
-      Gamma & {{x --> T11}} |- t12 ∈ T12 →
-      Gamma |- tabs x T11 t12 ∈ TArrow T11 T12
-  | T_App : ∀ T11 T12 Gamma t1 t2,
-      Gamma |- t1 ∈ TArrow T11 T12 →
-      Gamma |- t2 ∈ T11 →
-      Gamma |- tapp t1 t2 ∈ T12
-  | T_True : ∀ Gamma,
-       Gamma |- ttrue ∈ TBool
-  | T_False : ∀ Gamma,
-       Gamma |- tfalse ∈ TBool
-  | T_If : ∀ t1 t2 t3 T Gamma,
-       Gamma |- t1 ∈ TBool →
-       Gamma |- t2 ∈ T →
-       Gamma |- t3 ∈ T →
-       Gamma |- tif t1 t2 t3 ∈ T
-
-where "Gamma '|-' t '∈' T" := (has_type Gamma t T).
-
-Hint Constructors has_type.
 
 Program Definition Lambda : Category := {|
   obj     := type;
-  hom     := fun x y => ∀ var : type -> Type, Lam var (Func x y);
-  homset  := fun x y => {| equiv := fun f g =>
-    ∀ v, lamD v (f _) = lamD v (g _)
-  |};
-  id      := fun x => fun v => \ v : x, ^ Here;
-  compose := fun x y z f g => fun v => Abs (f (Scope v x) @ (g (Scope v x) @ (^ Here)));
+  hom     := fun x y => ∃ Γ (t : preterm), Typing Γ t (x --> y);
+  homset  := fun x y => {| equiv := fun f g => _ |};
+  id      := fun x => (_; (_; identity _ x));
+  compose := fun x y z f g =>
+    (_; (_; composition _ _ _ _ _ _ (`2`2 f) (`2`2 g)))
 |}.
-Next Obligation.
-  equivalence.
-  congruence.
-Qed.
-Next Obligation.
-  proper.
-  rewrite H.
-  rewrite H0.
-  reflexivity.
-Qed.
-Next Obligation.
-  simpl.
+Admit Obligations.
